\documentclass{article}
\usepackage{amsthm}
\usepackage{amsmath}
\newtheorem{theorem}{Theorem}[section]
\begin{document}
\begin{theorem}
\label{gaussian_value}
  $$G = \int_{-\infty}^{\infty}e^{-\frac{1}{2}x^2}dx = \sqrt{2\pi}$$
\end{theorem}
\begin{proof}
  \begin{align*}
    G^2 &= \left(\int_{-\infty}^{\infty}e^{-\frac{1}{2}x^2}dx\right)\int_{-\infty}^{\infty}e^{-\frac{1}{2}y^2}dy \\
&=  \int_{-\infty}^{\infty}\int_{-\infty}^{\infty}e^{-\frac{1}{2}(x^2 + y^2)}dxdy  \\
\intertext{Substitute $r=x^2+y^2$, $r\sin\theta=y$, $r\cos\theta=x$, hence $dxdy=rdrd\theta$}
G^2 &=\int_{0}^{2\pi}\int_{0}^{\infty}e^{-\frac{1}{2}r^2}rdrd\theta \\
&=\left[\theta\int_{0}^{\infty}re^{-\frac{1}{2}r^2}dr\right]_{\theta=0}^{\theta=2\pi} \\
&= 2\pi\left[-e^{-\frac{1}{2}r^2}\right]_{0}^{\infty} \\
&= 2\pi
  \end{align*}
Hence $G = \sqrt{2\pi}$
\end{proof}

\begin{theorem}
For $a^2$ real and positive.
  $$I = \int_{-\infty}^{\infty}e^{-a^2x^2 + bx + c}dx = \frac{\sqrt{\pi}}{a}e^{c + \frac{b^2}{4a^2}}$$
\end{theorem}
\begin{proof}
First, ``complete the square'' in the exponent by defining $r$, $s$ and $t$ by the equation:
$$ -a^2x^2 + bx + c = -\frac{(rx + s)^2}{2} + t$$
This gives us:
  \begin{align*}
    -r^2 &= -2a^2 &\Rightarrow r&=a\sqrt{2} \\
-rs &= b &\Rightarrow s&=\frac{-b}{a\sqrt{2}} \\
t - \frac{s^2}{2} &= c &\Rightarrow t&= \frac{b^2}{4a^2}
  \end{align*}
Using the completed square in the integral $I$:
\begin{align}
  I & = \int_{-\infty}^{\infty}e^{-\frac{(rx + s)^2}{2}+t}dx \\
&= e^t\int_{-\infty}^{\infty}e^{-\frac{(rx + s)^2}{2}}dx \\
\intertext{By assumption $a$ is real and positive, hence $r$ is also real and positive. We can therefore substitute $y = rx + s$ without changing the limits of the integration. With this substitution $\frac{dy}{r} = dx$.}
& = e^t\int_{-\infty}^{\infty}e^{-\frac{y^2}{2}}\frac{dy}{r} \\
&= \frac{e^t}{r}\int_{-\infty}^{\infty}e^{-\frac{y^2}{2}}dy \\
\intertext{Applying theorem \ref{gaussian_value} we have}
&= \frac{\sqrt{2\pi}}{r}e^t \\
\intertext{Subsituting in for $r$ and $t$}
&= \frac{\sqrt{\pi}}{a}e^{c+\frac{b^2}{4a^2}}
\end{align}
\end{proof}
\end{document}
